Proved quote_type

unquote.v
@@ -1,373 +1,9 @@
-Require Import Ascii.
+Require Import lang.
 Require Import lib.
 
-Inductive type: Type :=
-  | type_forall: ascii -> type -> type
-  | type_func: type -> type -> type
-  | type_var: ascii -> type.
 
-Inductive exp: Type :=
-  | exp_func: ascii -> type -> exp -> exp
-  | exp_app: exp -> exp -> exp
-  | exp_tfunc: ascii -> exp -> exp
-  | exp_tapp: exp -> type -> exp
-  | exp_var: ascii -> exp.
-
-Definition type_eq_dec: forall t1 t2: type, {t1 = t2} + {t1 <> t2}.
-Proof.
-  decide equality; apply ascii_dec.
-Defined.
-
-Definition mapping (A: Type) := ascii -> option A.
-
-Definition empty_mapping {A: Type} : mapping A :=
-  fun _ => None.
-
-Definition mapping_update {A: Type} (m: mapping A)
-           (k: ascii) (v: A) : mapping A :=
-  fun x => if ascii_dec x k then (Some v) else m x.
-
-Notation "{ k , v | m }" := (mapping_update m k v)
-                            (at level 0, v at level 0).
-
-Definition type_env := mapping type.
-
-Fixpoint subst_type (t: type) (id: ascii) (t': type) : type :=
-  match t with
-  | type_forall v t1 =>
-      if ascii_dec id v
-      then type_forall v t1
-      else type_forall v (subst_type t1 id t')
-  | type_func t1 t2 =>
-      type_func (subst_type t1 id t')
-                (subst_type t2 id t')
-  | type_var v => if ascii_dec id v then t' else t
-  end.
-
-Inductive type_subst_in_exp: exp -> ascii -> type -> exp -> Prop :=
-  | tse_func: forall v t_v t_v' e1 e1' id t',
-      subst_type t_v id t' = t_v' ->
-      type_subst_in_exp e1 id t' e1' ->
-      type_subst_in_exp (exp_func v t_v e1)
-                        id t' (exp_func v t_v' e1')
-  | tse_app: forall e1 e1' e2 e2' id t',
-      type_subst_in_exp e1 id t' e1' ->
-      type_subst_in_exp e2 id t' e2' ->
-      type_subst_in_exp (exp_app e1 e2) id t'
-                        (exp_app e1' e2')
-  | tse_tfunc_p: forall v e1 e1' id t',
-      v <> id ->
-      type_subst_in_exp e1 id t' e1' ->
-      type_subst_in_exp (exp_tfunc v e1) id t'
-                        (exp_tfunc v e1')
-  | tse_tfunc_n: forall e1 id t',
-      type_subst_in_exp (exp_tfunc id e1) id t'
-                        (exp_tfunc id e1)
-  | tse_tapp: forall e e' t1 t1' id t',
-      type_subst_in_exp e id t' e' ->
-      subst_type t1 id t' = t1' ->
-      type_subst_in_exp (exp_tapp e t1) id t'
-                        (exp_tapp e' t1')
-  | tse_var: forall v id t',
-      type_subst_in_exp (exp_var v) id t' (exp_var v).
-Hint Constructors type_subst_in_exp.
-
-Lemma type_subst_in_exp_total: forall e id t,
-    exists e', type_subst_in_exp e id t e'.
-Proof.
-  intros e id t.
-  induction e; try destruct IHe as [e' IHe].
-  - exists (exp_func a (subst_type t0 id t) e').
-    auto.
-  - destruct IHe1 as [e1' IHe1].
-    destruct IHe2 as [e2' IHe2].
-    exists (exp_app e1' e2'). auto.
-  - destruct (ascii_dec a id).
-    + subst. exists (exp_tfunc id e). auto.
-    + exists (exp_tfunc a e'). constructor; auto.
-  - exists (exp_tapp e' (subst_type t0 id t)). auto.
-  - exists (exp_var a). auto.
-Qed.
-
-
-Inductive exp_subst: exp -> ascii -> exp -> exp -> Prop :=
-  | es_func_p: forall v t_v e1 e1' id e',
-      v <> id ->
-      exp_subst e1 id e' e1' ->
-      exp_subst (exp_func v t_v e1) id e'
-                (exp_func v t_v e1')
-  | es_func_n: forall v t_v e1 e',
-      exp_subst (exp_func v t_v e1) v e'
-                (exp_func v t_v e1)
-  | es_app: forall e1 e1' e2 e2' id e',
-      exp_subst e1 id e' e1' ->
-      exp_subst e2 id e' e2' ->
-      exp_subst (exp_app e1 e2) id e'
-                (exp_app e1' e2')
-  | es_tfunc: forall v e1 e1' id e',
-      exp_subst e1 id e' e1' ->
-      exp_subst (exp_tfunc v e1) id e'
-                (exp_tfunc v e1')
-  | es_tapp: forall e1 e1' t id e',
-      exp_subst e1 id e' e1' ->
-      exp_subst (exp_tapp e1 t) id e'
-                (exp_tapp e1' t)
-  | es_var_p: forall id e',
-      exp_subst (exp_var id) id e' e'
-  | es_var_n: forall id1 id2 e',
-      id1 <> id2 ->
-      exp_subst (exp_var id1) id2 e' (exp_var id1).
-Hint Constructors exp_subst.
-
-Lemma exp_subst_total: forall e id e0,
-    exists e', exp_subst e id e0 e'.
-Proof.
-  intros e id e0.
-  induction e; try destruct IHe as [e' IHe].
-  - destruct (ascii_dec a id).
-    + exists (exp_func a t e). subst. auto.
-    + exists (exp_func a t e'). constructor; auto.
-  - destruct IHe1 as [e1' IHe1].
-    destruct IHe2 as [e2' IHe2].
-    exists (exp_app e1' e2'). auto.
-  - exists (exp_tfunc a e'). auto.
-  - exists (exp_tapp e' t). auto.
-  - destruct (ascii_dec a id); subst.
-    + exists e0. auto.
-    + exists (exp_var a). auto.
-Qed.
-
-
-Reserved Notation "env |- e : t"
-         (at level 40, e at level 39).
-
-Inductive type_checked: type_env -> exp -> type -> Prop :=
-  | tc_func: forall t_env v t_v e t_e,
-      { v, t_v | t_env } |- e : t_e ->
-      t_env |- (exp_func v t_v e) : (type_func t_v t_e)
-  | tc_app: forall t_env e1 e2 t_v t_e,
-      t_env |- e1 : (type_func t_v t_e) ->
-      t_env |- e2 : t_v ->
-      t_env |- (exp_app e1 e2) : t_e
-  | tc_tfunc: forall t_env v e t,
-      t_env |- e : t ->
-      t_env |- (exp_tfunc v e) : (type_forall v t)
-  | tc_tapp: forall t_env e v t_e t t_result,
-      t_env |- e : (type_forall v t_e) ->
-      subst_type t_e v t = t_result ->
-      t_env |- (exp_tapp e t) : t_result
-  | tc_var: forall t_env v t,
-      (t_env v) = (Some t) ->
-      t_env |- (exp_var v) : t
-where "env |- e : t" := (type_checked env e t).
-Hint Constructors type_checked.
-
-Reserved Notation "e1 |> e2"
-         (at level 40).
-
-Inductive beta_reduction: exp -> exp -> Prop :=
-  | br_func: forall v t_v e1 e1',
-      e1 |> e1' ->
-      (exp_func v t_v e1) |> (exp_func v t_v e1')
-  | br_app_full: forall v t_v e_f e_f' e2,
-      exp_subst e_f v e2 e_f' ->
-      (exp_app (exp_func v t_v e_f) e2) |> e_f'
-  | br_app_partial1: forall e1 e2 e1',
-      e1 |> e1' ->
-      (exp_app e1 e2) |> (exp_app e1' e2)
-  | br_app_partial2: forall e1 e2 e2',
-      e2 |> e2' ->
-      (exp_app e1 e2) |> (exp_app e1 e2')
-  | br_tfunc: forall v e1 e1',
-      e1 |> e1' ->
-      (exp_tfunc v e1) |> (exp_tfunc v e1')
-  | br_tapp_full: forall v e2 e2' t,
-      type_subst_in_exp e2 v t e2' ->
-      (exp_tapp (exp_tfunc v e2) t) |> e2'
-  | br_tapp_partial: forall e1 e1' t,
-      e1 |> e1' ->
-      (exp_tapp e1 t) |> (exp_tapp e1' t)
-where "e1 |> e2" := (beta_reduction e1 e2).
-Hint Constructors beta_reduction.
-
-Reserved Notation "e1 |>* e2"
-         (at level 40).
-
-Inductive beta_reductions: exp -> exp -> Prop :=
-  | bn_step: forall e1 e2 e3,
-      e1 |> e2 ->
-      e2 |>* e3 ->
-      e1 |>* e3
-  | bn_refl: forall e1,
-      e1 |>* e1
-where "e1 |>* e2" := (beta_reductions e1 e2).
-Hint Constructors beta_reductions.
-
-Inductive nf: exp -> Prop :=
-  | nf_func: forall v t_v e1,
-      nf e1 ->
-      nf (exp_func v t_v e1)
-  | nf_app: forall e1 e2,
-      nf e1 ->
-      nf e2 ->
-      (~ exists v t_v e', e1 = (exp_func v t_v e')) ->
-      nf (exp_app e1 e2)
-  | nf_tfunc: forall v e1,
-      nf e1 ->
-      nf (exp_tfunc v e1)
-  | nf_tapp: forall e1 t,
-      nf e1 ->
-      (~ exists v e', e1 = (exp_tfunc v e')) ->
-      nf (exp_tapp e1 t)
-  | nf_var: forall v,
-      nf (exp_var v).
-Hint Constructors nf.
-
-Fact nf_iff_stuck : forall e,
-    nf e <-> ~ exists e', beta_reduction e e'.
-Proof.
-  split.
-  - intros H.
-    induction e; intros [e' contra]; inversion H; subst;
-      try (apply (IHe H1);
-           inversion contra; subst;
-           exists e1'; auto).
-    + inversion contra; subst.
-      * apply H4. exists v, t_v, e_f. reflexivity.
-      * apply (IHe1 H2). exists e1'. auto.
-      * apply (IHe2 H3). exists e2'. auto.
-    + inversion contra; subst.
-      * apply H3. exists v, e2. reflexivity.
-      * apply (IHe H2). exists e1'. auto.
-    + inversion contra.
-  - intros H0.
-    induction e; constructor.
-    + apply IHe.
-      intros [e' contra].
-      apply H0.
-      exists (exp_func a t e'). auto.
-    + apply IHe1.
-      intros [e' contra].
-      apply H0.
-      exists (exp_app e' e2). auto.
-    + apply IHe2.
-      intros [e' contra].
-      apply H0.
-      exists (exp_app e1 e'). auto.
-    + intros [v [t_v [e' H]]]. subst.
-      apply H0.
-      destruct (exp_subst_total e' v e2) as [e H__subst].
-      exists e. auto.
-    + apply IHe.
-      intros [e' contra].
-      apply H0.
-      exists (exp_tfunc a e'). auto.
-    + apply IHe.
-      intros [e' contra].
-      apply H0.
-      exists (exp_tapp e' t). auto.
-    + intros [v [e' H]]. subst.
-      apply H0.
-      destruct (type_subst_in_exp_total e' v t) as [e'' H__subst].
-      exists e''. auto.
-Qed.
-
-
-Definition equivalent (e1 e2: exp) : Prop :=
-  exists e', (e1 |>* e') /\ (e2 |>* e').
-
-Notation "e1 ~ e2" := (equivalent e1 e2)
-                        (at level 20).
-
-
-Fixpoint _typecheck (t_env: type_env) (e: exp) : option type :=
-  match e with
-  | exp_func v t_v e =>
-      let new_t_env := { v, t_v | t_env } in
-      match _typecheck new_t_env e with
-      | Some t => Some (type_func t_v t)
-      | None => None
-      end
-  | exp_app e1 e2 =>
-      match (_typecheck t_env e1), (_typecheck t_env e2) with
-      | Some (type_func t1 t2), Some t3 =>
-          if type_eq_dec t1 t3
-          then Some t2
-          else None
-      | _, _ => None
-      end
-  | exp_tfunc v e =>
-      match _typecheck t_env e with
-      | Some t => Some (type_forall v t)
-      | None => None
-      end
-  | exp_tapp e1 t2 =>
-      match _typecheck t_env e1 with
-      | Some (type_forall v t1) =>
-          Some (subst_type t1 v t2)
-      | _ => None
-      end
-  | exp_var v => t_env v
-  end.
-
-Definition typecheck (e: exp) : option type :=
-  _typecheck empty_mapping e.
-
-Definition identity : exp :=
-  (exp_tfunc "t" (exp_func "x" (type_var "t") (exp_var "x"))).
-
-Definition identity_type :=
-  type_forall "t" (type_func (type_var "t") (type_var "t")).
-
-Fact identity_typechecked :
-  Some identity_type = typecheck identity.
-Proof.
-  compute. reflexivity.
-Qed.
-
-Theorem typecheck_sound : forall env e t,
-    _typecheck env e = Some t -> type_checked env e t.
-Proof.
-  intros env e. generalize dependent env.
-  induction e; intros env t' H0; simpl in H0.
-  - remember {a, t | env} as env'.
-    remember (_typecheck env' e) as ot.
-    destruct ot; inversion H0.
-    apply tc_func.
-    rewrite <- Heqenv'.
-    auto.
-  - remember (_typecheck env e1) as ot1.
-    remember (_typecheck env e2) as ot2.
-    destruct ot1 as [t1|];
-      try solve by inversion;
-      destruct t1 as [|t1 t0|]; try solve by inversion.
-    destruct ot2 as [t2|];
-      try solve by inversion.
-    destruct (type_eq_dec t1 t2); try solve by inversion.
-    inversion H0. subst.
-    apply tc_app with t2; auto.
-  - remember (_typecheck env e) as ot.
-    destruct ot as [t|]; try solve by inversion.
-    inversion H0. subst.
-    apply tc_tfunc. auto.
-  - remember (_typecheck env e) as ot.
-    destruct ot as [t0|]; try solve by inversion.
-    destruct t0; try solve by inversion.
-    inversion H0. subst.
-    apply tc_tapp with a t0; auto.
-  - auto.
-Qed.
-
-Theorem typecheck_complete : forall env e t,
-    type_checked env e t -> _typecheck env e = Some t.
-Proof.
-  intros env e t H0.
-  induction H0; simpl; try rewrite IHtype_checked; try reflexivity.
-  - rewrite IHtype_checked1. rewrite IHtype_checked2.
-    destruct (type_eq_dec t_v t_v) as [b|b]; try elim b; reflexivity.
-  - subst. reflexivity.
-  - auto.
-Qed.
+Definition injection_symbol : ascii := "i".
+Definition injection_var : exp := (exp_var "i").
 
 Fixpoint _quote (t_env: type_env) (e: exp) : option exp :=
   match e with
@@ -381,7 +17,7 @@ Fixpoint _quote (t_env: type_env) (e: exp) : option exp :=
             _quote t_env e2 with
       | Some t, Some e1', Some e2' =>
           Some (exp_app (exp_app
-                           (exp_tapp (exp_var "i") t) e1'
+                           (exp_tapp injection_var t) e1'
                         ) e2')
       | _, _, _ => None
       end 
@@ -391,9 +27,9 @@ Fixpoint _quote (t_env: type_env) (e: exp) : option exp :=
   | exp_tapp e t =>
       match _typecheck t_env e,
             _quote t_env e with
-      | Some t, Some e' =>
+      | Some t', Some e' =>
           Some (exp_tapp (exp_app
-                            (exp_tapp (exp_var "i") t) e'
+                            (exp_tapp injection_var t') e'
                          ) t)
       | _, _ => None
       end
@@ -403,14 +39,13 @@ Fixpoint _quote (t_env: type_env) (e: exp) : option exp :=
 Hint Transparent option_map.
 
 Definition quote (e: exp) : option exp :=
-  option_map (fun e' => exp_func "i" identity_type e')
+  option_map (fun e' => exp_func injection_symbol identity_type e')
              (_quote empty_mapping e).
 
 Definition unquote : exp :=
   let rtype := type_func identity_type (type_var "a") in
   exp_tfunc "a" (exp_func "q" rtype
                           (exp_app (exp_var "q") identity)).
-
 
 Lemma strong_quote_nf : forall e e' t_env,
     _quote t_env e = Some e' ->
@@ -455,6 +90,7 @@ Proof.
     auto.
 Qed.
 
+
 Theorem quote_nf : forall e e',
     quote e = Some e' ->
     nf e'.
@@ -469,11 +105,113 @@ Proof.
   auto.
 Qed.
 
-Theorem quote_type : forall e e' t,
-    quote e = Some e' ->
-    typecheck e = Some t ->
-    typecheck e' = Some (type_func identity_type t).
+
+Inductive no_injection_symbol : exp -> Prop :=
+  | nis_func: forall v t_v e,
+      v <> injection_symbol ->
+      no_injection_symbol e ->
+      no_injection_symbol (exp_func v t_v e)
+  | nis_app: forall e1 e2,
+      no_injection_symbol e1 ->
+      no_injection_symbol e2 ->
+      no_injection_symbol (exp_app e1 e2)
+  | nis_tfunc: forall v e,
+      no_injection_symbol e ->
+      no_injection_symbol (exp_tfunc v e)
+  | nis_tapp: forall e t,
+      no_injection_symbol e ->
+      no_injection_symbol (exp_tapp e t)
+  | nis_var: forall v,
+      v <> injection_symbol ->
+      no_injection_symbol (exp_var v).
+
+
+Lemma strong_quote_type : forall e e' env t0,
+    no_injection_symbol e ->
+    _quote env e = Some e' ->
+    _typecheck env e = Some t0 ->
+    _typecheck {injection_symbol, identity_type | env} e'
+    = Some t0.
 Proof.
+  intros e e' env t0 Hi He Ht.
+  apply typecheck_sound in Ht.
+  apply typecheck_complete.
+  generalize dependent e'.
+  generalize dependent env.
+  generalize dependent t0.
+  induction e; intros t0 env Ht e0' He; simpl in He;
+    try unfold option_map in He;
+    inversion Ht; subst; inversion Hi.
+  - remember {a, t | env} as new_env.
+    remember (_quote new_env e) as oe'.
+    destruct oe' as [e'|]; inversion He.
+    constructor.
+    rewrite (mapping_reorder _ _ _ _ _ H1).
+    rewrite <- Heqnew_env.
+    auto.
+  - remember (_typecheck env e1) as ot1.
+    remember (_quote env e1) as oe1'.
+    remember (_quote env e2) as oe2'.
+    destruct ot1 as [t1|]; inversion He.
+    destruct oe1' as [e1'|]; inversion He.
+    destruct oe2' as [e2'|]; inversion He.
+    subst.
+    apply tc_app with t_v;
+      try apply tc_app with (type_func t_v t0);
+      try apply tc_tapp with
+      identity_type_symbol identity_inner_type;
+      auto.
+    (* i t1 |- t1 -> t1 *)
+    apply typecheck_complete in H2.
+    rewrite H2 in Heqot1.
+    inversion Heqot1.
+    auto.
+  - remember (_quote env e) as oe'.
+    destruct oe' as [e'|]; inversion He.
+    auto.
+  - remember (_typecheck env e) as ot'.
+    remember (_quote env e) as oe'.
+    destruct ot' as [t'|]; inversion He.
+    destruct oe' as [e'|]; inversion He.
+    apply tc_tapp with v t_e; auto.
+    apply tc_app with (type_forall v t_e); auto.
+    apply tc_tapp with
+    identity_type_symbol identity_inner_type; auto.
+    apply typecheck_complete in H2.
+    rewrite H2 in Heqot'.
+    inversion Heqot'.
+    auto.
+  - inversion He.
+    constructor.
+    unfold mapping_update.
+    destruct (ascii_dec a injection_symbol).
+    + contradiction.
+    + auto.
+Qed.
+
+
+Theorem quote_type : forall e e' t0,
+    no_injection_symbol e ->
+    quote e = Some e' ->
+    typecheck e = Some t0 ->
+    typecheck e' = Some (type_func identity_type t0).
+Proof.
+  intros e e' t0 H0 H1.
+  unfold quote in H1.
+  unfold option_map in H1.
+  remember (_quote empty_mapping e) as oe'.
+  destruct oe'; destruct e'; inversion H1.
+  subst. clear H1.
+  intros H2.
+  apply typecheck_complete.
+  constructor.
+  apply typecheck_sound.
+  eapply strong_quote_type.
+  apply H0.
+  auto.
+  auto.
+Qed.
+
 
 Theorem unquoted_eq : forall e e' t,
     quote e = Some e' ->
